Use sets instead of lists for Lem nondeterminism monad
This simplifies reasoning in Isabelle.

lib/isabelle/State_monad_lemmas.thy
@@ -8,34 +8,36 @@ context
   notes returnS_def[simp] and failS_def[simp] and throwS_def[simp] and readS_def[simp] and updateS_def[simp]
 begin
 
-abbreviation "bindS_aux f \<equiv> (\<lambda>r. case r of (Value a, s') \<Rightarrow> f a s' | (Ex e, s') \<Rightarrow> [(Ex e, s')])"
-abbreviation "bindS_app ms f \<equiv> List.concat (List.map (bindS_aux f) ms)"
+abbreviation "bindS_aux f \<equiv> (\<lambda>r. case r of (Value a, s') \<Rightarrow> f a s' | (Ex e, s') \<Rightarrow> {(Ex e, s')})"
+abbreviation "bindS_app ms f \<equiv> \<Union>(bindS_aux f ` ms)"
 
 lemma bindS_ext_cong[fundef_cong]:
   assumes m: "m1 s = m2 s"
-    and f: "\<And>a s'. (Value a, s') \<in> set (m2 s) \<Longrightarrow> f1 a s' = f2 a s'"
+    and f: "\<And>a s'. (Value a, s') \<in> (m2 s) \<Longrightarrow> f1 a s' = f2 a s'"
   shows "bindS m1 f1 s = bindS m2 f2 s"
-proof -
+  using assms unfolding bindS_def by (auto split: result.splits)
+(* proof -
   have "bindS_app (m2 s) f1 = bindS_app (m2 s) f2"
-    using f by (intro arg_cong[where f = List.concat]) (auto intro: map_ext split: result.splits)
+    using f by (auto split: result.splits)
   then show ?thesis using m by (auto simp: bindS_def)
-qed
+qed *)
 
 lemma bindS_cong[fundef_cong]:
   assumes m: "m1 = m2"
-    and f: "\<And>s a s'. (Value a, s') \<in> set (m2 s) \<Longrightarrow> f1 a s' = f2 a s'"
+    and f: "\<And>s a s'. (Value a, s') \<in> (m2 s) \<Longrightarrow> f1 a s' = f2 a s'"
   shows "bindS m1 f1 = bindS m2 f2"
-  using assms by (blast intro: bindS_ext_cong)
+  using assms by (intro ext bindS_ext_cong; blast)
 
 lemma bindS_returnS_left[simp]: "bindS (returnS x) f = f x"
   by (auto simp add: bindS_def)
 
 lemma bindS_returnS_right[simp]: "bindS m returnS = (m :: ('regs, 'a, 'e) monadS)"
-proof -
+  by (intro ext) (auto simp: bindS_def split: result.splits)
+(* proof -
   have "List.concat (map (bindS_aux returnS) ms) = ms" for ms :: "(('a, 'e) result \<times> 'regs sequential_state) list"
     by (induction ms) (auto split: result.splits)
   then show ?thesis unfolding bindS_def by blast
-qed
+qed *)
 
 lemma bindS_readS: "bindS (readS f) m = (\<lambda>s. m (f s) s)"
   by (auto simp: bindS_def)
@@ -43,30 +45,100 @@ lemma bindS_readS: "bindS (readS f) m = (\<lambda>s. m (f s) s)"
 lemma bindS_updateS: "bindS (updateS f) m = (\<lambda>s. m () (f s))"
   by (auto simp: bindS_def)
 
-lemma bindS_assoc[simp]: "bindS (bindS m f) g = bindS m (\<lambda>x. bindS (f x) g)"
+
+lemma result_cases:
+  fixes r :: "('a, 'e) result"
+  obtains (Value) a where "r = Value a"
+  | (Throw) e where "r = Ex (Throw e)"
+  | (Failure) msg where "r = Ex (Failure msg)"
+proof (cases r)
+  case (Ex ex) then show ?thesis by (cases ex; auto intro: that)
+qed
+
+lemma result_state_cases:
+  fixes rs :: "('a, 'e) result \<times> 's"
+  obtains (Value) a s where "rs = (Value a, s)"
+  | (Throw) e s where "rs = (Ex (Throw e), s)"
+  | (Failure) msg s where "rs = (Ex (Failure msg), s)"
 proof -
+  obtain r s where rs: "rs = (r, s)" by (cases rs)
+  then show thesis by (cases r rule: result_cases) (auto intro: that)
+qed
+
+lemma monadS_ext_eqI:
+  fixes m m' :: "('regs, 'a, 'e) monadS"
+  assumes "\<And>a s'. (Value a, s') \<in> m s \<longleftrightarrow> (Value a, s') \<in> m' s"
+    and "\<And>e s'. (Ex (Throw e), s') \<in> m s \<longleftrightarrow> (Ex (Throw e), s') \<in> m' s"
+    and "\<And>msg s'. (Ex (Failure msg), s') \<in> m s \<longleftrightarrow> (Ex (Failure msg), s') \<in> m' s"
+  shows "m s = m' s"
+proof (intro set_eqI)
+  fix x
+  show "x \<in> m s \<longleftrightarrow> x \<in> m' s" using assms by (cases x rule: result_state_cases) auto
+qed
+
+lemma monadS_eqI:
+  fixes m m' :: "('regs, 'a, 'e) monadS"
+  assumes "\<And>s a s'. (Value a, s') \<in> m s \<longleftrightarrow> (Value a, s') \<in> m' s"
+    and "\<And>s e s'. (Ex (Throw e), s') \<in> m s \<longleftrightarrow> (Ex (Throw e), s') \<in> m' s"
+    and "\<And>s msg s'. (Ex (Failure msg), s') \<in> m s \<longleftrightarrow> (Ex (Failure msg), s') \<in> m' s"
+  shows "m = m'"
+  using assms by (intro ext monadS_ext_eqI)
+
+lemma
+  assumes "(Value a, s') \<in> bindS m f s"
+  obtains a' s'' where "(Value a', s'') \<in> m s" and "(Value a, s') \<in> f a' s''"
+  using assms by (auto simp: bindS_def split: result.splits)
+
+lemma
+  assumes "(Ex e, s') \<in> bindS m f s"
+  obtains (Left) "(Ex e, s') \<in> m s"
+  | (Right) a s'' where "(Value a, s'') \<in> m s" and "(Ex e, s') \<in> f a s''"
+  using assms by (auto simp: bindS_def split: result.splits)
+
+lemma bindS_cases:
+  assumes "(r, s') \<in> bindS m f s"
+  obtains (Value) a a' s'' where "r = Value a" and "(Value a', s'') \<in> m s" and "(Value a, s') \<in> f a' s''"
+  | (Ex_Left) e where "r = Ex e" and "(Ex e, s') \<in> m s"
+  | (Ex_Right) e a s'' where "r = Ex e" and "(Value a, s'') \<in> m s" and "(Ex e, s') \<in> f a s''"
+  using assms by (cases r; auto simp: bindS_def split: result.splits)
+
+lemma bindS_intros:
+  "\<And>m f s a s' a' s''. (Value a', s'') \<in> m s \<Longrightarrow> (Value a, s') \<in> f a' s'' \<Longrightarrow> (Value a, s') \<in> bindS m f s"
+  "\<And>m f s e s'. (Ex e, s') \<in> m s \<Longrightarrow> (Ex e, s') \<in> bindS m f s"
+  "\<And>m f s e s' a s''. (Ex e, s') \<in> f a s'' \<Longrightarrow> (Value a, s'') \<in> m s \<Longrightarrow> (Ex e, s') \<in> bindS m f s"
+  by (auto simp: bindS_def intro: bexI[rotated])
+
+lemma bindS_assoc[simp]: "bindS (bindS m f) g = bindS m (\<lambda>x. bindS (f x) g)"
+  by (auto elim!: bindS_cases intro: bindS_intros monadS_eqI)
+(*proof -
   have "List.concat (map (bindS_aux g) (List.concat (map (bindS_aux f) xs))) =
         List.concat (map (bindS_aux (\<lambda>x s. List.concat (map (bindS_aux g) (f x s)))) xs)" for xs
     by (induction xs) (auto split: result.splits)
   then show ?thesis unfolding bindS_def by auto
-qed
+qed*)
 
 lemma bindS_failS[simp]: "bindS (failS msg) f = failS msg" by (auto simp: bindS_def)
 lemma bindS_throwS[simp]: "bindS (throwS e) f = throwS e" by (auto simp: bindS_def)
 declare seqS_def[simp]
 
 lemma Value_bindS_elim:
-  assumes "(Value a, s') \<in> set (bindS m f s)"
-  obtains s'' a' where "(Value a', s'') \<in> set (m s)" and "(Value a, s') \<in> set (f a' s'')"
-  using assms by (auto simp: bindS_def; split result.splits; auto)
+  assumes "(Value a, s') \<in> bindS m f s"
+  obtains s'' a' where "(Value a', s'') \<in> m s" and "(Value a, s') \<in> f a' s''"
+  using assms by (auto elim: bindS_cases)
+
+lemma Ex_bindS_elim:
+  assumes "(Ex e, s') \<in> bindS m f s"
+  obtains (Left) "(Ex e, s') \<in> m s"
+  | (Right) s'' a' where "(Value a', s'') \<in> m s" and "(Ex e, s') \<in> f a' s''"
+  using assms by (auto elim: bindS_cases)
 
 abbreviation
   "try_catchS_aux h r \<equiv>
     (case r of
        (Value a, s') => returnS a s'
      | (Ex (Throw e), s') => h e s'
-     | (Ex (Failure msg), s') => [(Ex (Failure msg), s')])"
-abbreviation "try_catchS_app ms h \<equiv> List.concat (List.map (try_catchS_aux h) ms)"
+     | (Ex (Failure msg), s') => {(Ex (Failure msg), s')})"
+abbreviation "try_catchS_app ms h \<equiv> \<Union>(try_catchS_aux h ` ms)"
 
 lemma try_catchS_returnS[simp]: "try_catchS (returnS a) h = returnS a"
   and try_catchS_failS[simp]: "try_catchS (failS msg) h = failS msg"
@@ -78,6 +150,31 @@ lemma try_catchS_cong[cong]:
   shows "try_catchS m1 h1 = try_catchS m2 h2"
   using assms by (intro arg_cong2[where f = try_catchS] ext) auto
 
+lemma try_catchS_cases:
+  assumes "(r, s') \<in> try_catchS m h s"
+  obtains (Value) a where "r = Value a" and "(Value a, s') \<in> m s"
+  | (Fail) msg where "r = Ex (Failure msg)" and "(Ex (Failure msg), s') \<in> m s"
+  | (h) e s'' where "(Ex (Throw e), s'') \<in> m s" and "(r, s') \<in> h e s''"
+  using assms by (cases r rule: result_cases) (auto simp: try_catchS_def split: result.splits ex.splits)
+
+lemma try_catchS_intros:
+  "\<And>m h s a s'. (Value a, s') \<in> m s \<Longrightarrow> (Value a, s') \<in> try_catchS m h s"
+  "\<And>m h s msg s'. (Ex (Failure msg), s') \<in> m s \<Longrightarrow> (Ex (Failure msg), s') \<in> try_catchS m h s"
+  "\<And>m h s e s'' r s'. (Ex (Throw e), s'') \<in> m s \<Longrightarrow> (r, s') \<in> h e s'' \<Longrightarrow> (r, s') \<in> try_catchS m h s"
+  by (auto simp: try_catchS_def intro: bexI[rotated])
+
+fun ignore_throw_aux :: "(('a, 'e1) result \<times> 's) \<Rightarrow> (('a, 'e2) result \<times> 's) set" where
+  "ignore_throw_aux (Value a, s') = {(Value a, s')}"
+| "ignore_throw_aux (Ex (Throw e), s') = {}"
+| "ignore_throw_aux (Ex (Failure msg), s') = {(Ex (Failure msg), s')}"
+definition "ignore_throw m s \<equiv> \<Union>(ignore_throw_aux ` m s)"
+
+(*fun ignore_throw_aux :: "(('a, 'e1) result \<times> 's) \<Rightarrow> (('a, 'e2) result \<times> 's) list" where
+  "ignore_throw_aux r \<equiv>
+    (case r of
+       (Value a, s') => returnS a s'
+     | (Ex (Throw e), s') => h e s'
+     | (Ex (Failure msg), s') => {(Ex (Failure msg), s')})"
 fun ignore_throw_app :: "(('a, 'e1) result \<times> 's) list \<Rightarrow> (('a, 'e2) result \<times> 's) list" where
   "ignore_throw_app [] = []"
 | "ignore_throw_app ((Value a, s) # ms) = (Value a, s) # ignore_throw_app ms"
@@ -95,12 +192,31 @@ lemma ignore_throw_app_append[simp]:
 
 lemma ignore_throw_app_bindS_app[simp]:
   "ignore_throw_app (bindS_app ms f) = bindS_app (ignore_throw_app ms) (ignore_throw \<circ> f)"
-  by (induction ms rule: ignore_throw_app.induct) (auto split: result.splits)
+  by (induction ms rule: ignore_throw_app.induct) (auto split: result.splits)*)
+
+lemma [simp]:
+  "(Value a, s') \<in> ignore_throw_aux ms \<longleftrightarrow> ms = (Value a, s')"
+  "(Ex (Throw e), s') \<in> ignore_throw_aux ms \<longleftrightarrow> False"
+  "(Ex (Failure msg), s') \<in> ignore_throw_aux ms \<longleftrightarrow> ms = (Ex (Failure msg), s')"
+  by (cases ms rule: result_state_cases; auto)+
+
+(*lemma [simp]: "(Value a, s') \<in> ignore_throw m s \<longleftrightarrow> (Value a, s') \<in> m s"
+  "(Value a, s') \<in> ignore_throw m s \<longleftrightarrow> (Value a, s') \<in> m s"
+  "(Ex (Throw e), s') \<in> ignore_throw m s \<longleftrightarrow> False"
+  "(Ex (Failure msg), s') \<in> ignore_throw_aux ms \<longleftrightarrow> ms = (Ex (Failure msg), s')"
+  by (auto simp: ignore_throw_def)*)
+
+lemma ignore_throw_cases:
+  assumes no_throw: "ignore_throw m s = m s"
+    and r: "(r, s') \<in> m s"
+  obtains (Value) a where "r = Value a"
+  | (Failure) msg where "r = Ex (Failure msg)"
+  using r unfolding no_throw[symmetric]
+  by (cases r rule: result_cases) (auto simp: ignore_throw_def)
 
 lemma ignore_throw_bindS[simp]:
   "ignore_throw (bindS m f) = bindS (ignore_throw m) (ignore_throw \<circ> f)"
-  "ignore_throw (bindS m f) s = bindS (ignore_throw m) (ignore_throw \<circ> f) s"
-  unfolding bindS_def by auto
+  by (intro monadS_eqI) (auto simp: ignore_throw_def elim!: bindS_cases intro: bindS_intros)
 
 lemma try_catchS_bindS_no_throw:
   fixes m1 :: "('r, 'a, 'e1) monadS" and m2 :: "('r, 'a, 'e2) monadS"
@@ -109,13 +225,47 @@ lemma try_catchS_bindS_no_throw:
   shows "try_catchS (bindS m1 f) h = bindS m2 (\<lambda>a. try_catchS (f a) h)"
 proof
   fix s
+  have "try_catchS (bindS m1 f) h s = bindS (ignore_throw m1) (\<lambda>a. try_catchS (f a) h) s"
+    by (intro monadS_ext_eqI;
+        auto elim!: bindS_cases try_catchS_cases elim: ignore_throw_cases[OF m1];
+        auto simp: ignore_throw_def intro: bindS_intros try_catchS_intros)
+  also have "\<dots> = bindS m2 (\<lambda>a. try_catchS (f a) h) s" using m2 by (intro bindS_ext_cong) auto
+  finally show "try_catchS (bindS m1 f) h s = bindS m2 (\<lambda>a. try_catchS (f a) h) s" .
+qed
+(*proof
+  fix s
   have 1: "try_catchS_app (bindS_app ms f) h =
         bindS_app (ignore_throw_app ms) (\<lambda>a s'. try_catchS_app (f a s') h)"
     if "ignore_throw_app ms = ms" for ms
     using that by (induction ms rule: ignore_throw_app.induct) auto
   then show "try_catchS (bindS m1 f) h s = bindS m2 (\<lambda>a. try_catchS (f a) h) s"
     using m1 unfolding try_catchS_def bindS_def m2[symmetric] by blast
-qed
+qed*)
+
+(*lemma no_throwI:
+  fixes m1 :: "('regs, 'a, 'e1) monadS" and m2 :: "('regs, 'a, 'e2) monadS"
+  assumes "\<And>a s'. (Value a, s') \<in> m1 s \<longleftrightarrow> (Value a, s') \<in> m2 s"
+    and "\<And>msg s'. (Ex (Failure msg), s') \<in> m1 s \<longleftrightarrow> (Ex (Failure msg), s') \<in> m2 s"
+    and "\<And>e s'. (Ex (Throw e), s') \<notin> m1 s"
+    and "\<And>e s'. (Ex (Throw e), s') \<notin> m2 s"
+  shows "ignore_throw m1 s = m2 s"
+  using assms by (intro monadS_ext_eqI) (auto simp: ignore_throw_def)*)
+
+(*lemma no_throw_bindSI:
+  assumes "ignore_throw m1 s = m2 s"
+and "\<And>a s'. (Value a, s') \<in> m2 s \<Longrightarrow> ignore_throw (f1 a) s' = f2 a s'"
+shows "ignore_throw (bindS m1 f1) s = bindS m2 f2 s"
+  using assms unfolding ignore_throw_bindS apply (intro monadS_ext_eqI) apply auto apply (auto elim!: bindS_cases intro: bindS_intros)
+   defer thm bindS_intros
+   apply (intro bindS_intros(3)) apply auto
+  apply (intro bindS_intros(3)) apply auto
+  done
+
+lemma
+  "\<And>BC rk a sz s. ignore_throw (read_mem_bytesS BC rk a sz) s = read_mem_bytesS BC rk a sz s"
+  unfolding read_mem_bytesS_def Let_def seqS_def
+  apply (intro no_throw_bindSI)
+  oops*)
 
 lemma no_throw_mem_builtins:
   "\<And>a. ignore_throw (returnS a) = returnS a"
@@ -130,16 +280,16 @@ lemma no_throw_mem_builtins:
   unfolding read_mem_bytesS_def read_memS_def read_tagS_def write_mem_eaS_def
   unfolding write_mem_valS_def write_mem_bytesS_def write_tagS_def
   unfolding excl_resultS_def undefined_boolS_def
-  by (auto simp: bindS_def chooseS_def Let_def split: option.splits prod.splits)+
+  by (auto simp: ignore_throw_def bindS_def chooseS_def Let_def split: option.splits prod.splits)
 
 lemma no_throw_read_memS: "ignore_throw (read_memS BCa BCb rk a sz) s = read_memS BCa BCb rk a sz s"
-  by (auto simp: read_memS_def no_throw_mem_builtins cong: bindS_cong)
+  by (auto simp: read_memS_def no_throw_mem_builtins cong: bindS_ext_cong)
 
 lemma no_throw_read_regvalS: "ignore_throw (read_regvalS r reg_name) s = read_regvalS r reg_name s"
-  by (cases r) (auto simp: bindS_def split: option.splits)
+  by (cases r) (auto simp: ignore_throw_def bindS_def split: option.splits)
 
 lemma no_throw_write_regvalS: "ignore_throw (write_regvalS r reg_name v) s = write_regvalS r reg_name v s"
-  by (cases r) (auto simp: bindS_def split: option.splits)
+  by (cases r) (auto simp: ignore_throw_def bindS_def split: option.splits)
 
 lemmas no_throw_builtins[simp, intro] =
   no_throw_mem_builtins no_throw_read_regvalS no_throw_write_regvalS no_throw_read_memS
